commit

AP/System/Symmetry/Defs.lean
@@ -21,60 +21,120 @@ theorem one_def : (1 : Symmetry sys) = one := rfl
 instance : Inhabited (Symmetry sys) := ⟨1⟩
 theorem default_eq : (default : Symmetry sys) = 1 := rfl
 
-#check 0 #exit
+def fs (sym : Symmetry sys) (s : S) [hs : sys.WF s] : S :=
+  sym.lift (·.fs s) # λ _ _ h => by exact h.hs
 
-@[simp] theorem fs'_fs {s} [hs : sys.WF s] : sym.fs' (sym.fs s) = s := Raw₀.fs'_fs
-@[simp] theorem fs_fs' {s} [hs : sys.WF s] : sym.fs (sym.fs' s) = s := Raw₀.fs_fs'
-@[simp] theorem ft'_ft {t} [ht : sys.WFTrans t] : sym.ft' (sym.ft t) = t := Raw₀.ft'_ft
-@[simp] theorem ft_ft' {t} [ht : sys.WFTrans t] : sym.ft (sym.ft' t) = t := Raw₀.ft_ft'
+def fs' (sym : Symmetry sys) (s : S) [hs : sys.WF s] : S :=
+  sym.lift (·.fs' s) # λ _ _ h => by exact h.hs'
 
-theorem tr_fs {s t} [hs : sys.WF s] :
-sys.tr (sym.fs s) t = (sys.tr s (sym.ft' t)).map sym.fs := Raw₀.tr_fs
+def ft (sym : Symmetry sys) (t : T) [ht : sys.WFTrans t] : T :=
+  sym.lift (·.ft t) # λ _ _ h => by exact h.ht
 
-theorem tr_fs' {s t} [hs : sys.WF s] :
-sys.tr (sym.fs' s) t = (sys.tr s (sym.ft t)).map sym.fs' := Raw₀.tr_fs'
+def ft' (sym : Symmetry sys) (t : T) [ht : sys.WFTrans t] : T :=
+  sym.lift (·.ft' t) # λ _ _ h => by exact h.ht'
 
-theorem tr_ft {s t} [hs : sys.WF s] :
-sys.tr s (sym.ft t) = (sys.tr (sym.fs' s) t).map sym.fs := Raw₀.tr_ft
+instance {s} [hs : sys.WF s] : sys.WF (sym.fs s) := by
+  apply sym.ind; simp [fs]; infer_instance
 
-theorem tr_ft' {s t} [hs : sys.WF s] :
-sys.tr s (sym.ft' t) = (sys.tr (sym.fs s) t).map sym.fs' := Raw₀.tr_ft'
+instance {s} [hs : sys.WF s] : sys.WF (sym.fs' s) := by
+  apply sym.ind; simp [fs']; infer_instance
 
-theorem validTr_fs_of {s t} [hs : sys.WF s]
-(h : sys.validTr s (sym.ft' t)) : sys.validTr (sym.fs s) t := Raw₀.validTr_fs_of h
+instance {t} [ht : sys.WFTrans t] : sys.WFTrans (sym.ft t) := by
+  apply sym.ind; simp [ft]; infer_instance
 
-theorem validTr_fs'_of {s t} [hs : sys.WF s]
-(h : sys.validTr s (sym.ft t)) : sys.validTr (sym.fs' s) t := Raw₀.validTr_fs'_of h
+instance {t} [ht : sys.WFTrans t] : sys.WFTrans (sym.ft' t) := by
+  apply sym.ind; simp [ft']; infer_instance
 
-theorem validTr_ft_of {s t} [hs : sys.WF s]
-(h : sys.validTr (sym.fs' s) t) : sys.validTr s (sym.ft t) := Raw₀.validTr_ft_of h
+@[simp]
+theorem fs'_fs {s} [hs : sys.WF s] : sym.fs' (sym.fs s) = s := by
+  apply sym.ind; simp [fs, fs']
 
-theorem validTr_ft'_of {s t} [hs : sys.WF s]
-(h : sys.validTr (sym.fs s) t) : sys.validTr s (sym.ft' t) := Raw₀.validTr_ft'_of h
+@[simp]
+theorem fs_fs' {s} [hs : sys.WF s] : sym.fs (sym.fs' s) = s := by
+  apply sym.ind; simp [fs, fs']
 
-theorem validTr_fs {s t} [hs : sys.WF s] :
-sys.validTr (sym.fs s) t ↔ sys.validTr s (sym.ft' t) := Raw₀.validTr_fs
+@[simp]
+theorem ft'_ft {t} [ht : sys.WFTrans t] : sym.ft' (sym.ft t) = t := by
+  apply sym.ind; simp [ft, ft']
 
-theorem validTr_fs' {s t} [hs : sys.WF s] :
-sys.validTr (sym.fs' s) t ↔ sys.validTr s (sym.ft t) := Raw₀.validTr_fs'
+@[simp]
+theorem ft_ft' {t} [ht : sys.WFTrans t] : sym.ft (sym.ft' t) = t := by
+  apply sym.ind; simp [ft, ft']
 
-theorem validTr_ft {s t} [hs : sys.WF s] :
-sys.validTr s (sym.ft t) ↔ sys.validTr (sym.fs' s) t := Raw₀.validTr_ft
+theorem tr_fs {s t} [hs : sys.WF s] [ht : sys.WFTrans t] :
+sys.tr (sym.fs s) t = match h : sys.tr s (sym.ft' t) with
+| none => none | some s' => haveI := wf_of_tr h; sym.fs s' := by
+  apply sym.ind; simp [fs, ft']; intro sym; rw [sym.tr_fs]; split <;> simp_all
 
-theorem validTr_ft' {s t} [hs : sys.WF s] :
+theorem tr_fs' {s t} [hs : sys.WF s] [ht : sys.WFTrans t] :
+sys.tr (sym.fs' s) t = match h : sys.tr s (sym.ft t) with
+| none => none | some s' => haveI := wf_of_tr h; sym.fs' s' := by
+  apply sym.ind; simp [fs', ft]; intro sym; rw [sym.tr_fs']; split <;> simp_all
+
+theorem tr_ft {s t} [hs : sys.WF s] [ht : sys.WFTrans t] :
+sys.tr s (sym.ft t) = match h : sys.tr (sym.fs' s) t with
+| none => none | some s' => haveI := wf_of_tr h; sym.fs s' := by
+  apply sym.ind; simp [fs, fs', ft]; intro sym; rw [sym.tr_ft]; split <;> simp_all
+
+theorem tr_ft' {s t} [hs : sys.WF s] [ht : sys.WFTrans t] :
+sys.tr s (sym.ft' t) = match h : sys.tr (sym.fs s) t with
+| none => none | some s' => haveI := wf_of_tr h; sym.fs' s' := by
+  apply sym.ind; simp [fs, fs', ft']; intro sym; rw [sym.tr_ft']; split <;> simp_all
+
+theorem validTr_fs_of {s t} [hs : sys.WF s] [ht : sys.WFTrans t]
+(h : sys.validTr s (sym.ft' t)) : sys.validTr (sym.fs s) t := by
+  obtain ⟨s', h⟩ := h; have h₁ := wf_of_tr h; use sym.fs s'
+  rw [tr_ft'] at h; split at h <;> simp_all; simp [←h]
+
+theorem validTr_fs'_of {s t} [hs : sys.WF s] [ht : sys.WFTrans t]
+(h : sys.validTr s (sym.ft t)) : sys.validTr (sym.fs' s) t := by
+  obtain ⟨s', h⟩ := h; have h₁ := wf_of_tr h; use sym.fs' s'
+  rw [tr_ft] at h; split at h <;> simp_all; simp [←h]
+
+theorem validTr_ft_of {s t} [hs : sys.WF s] [ht : sys.WFTrans t]
+(h : sys.validTr (sym.fs' s) t) : sys.validTr s (sym.ft t) := by
+  obtain ⟨s', h⟩ := h; have h₁ := wf_of_tr h; use sym.fs s'
+  rw [tr_fs'] at h; split at h <;> simp_all; simp [←h]
+
+theorem validTr_ft'_of {s t} [hs : sys.WF s] [ht : sys.WFTrans t]
+(h : sys.validTr (sym.fs s) t) : sys.validTr s (sym.ft' t) := by
+  obtain ⟨s', h⟩ := h; have h₁ := wf_of_tr h; use sym.fs' s'
+  rw [tr_fs] at h; split at h <;> simp_all; simp [←h]
+
+theorem validTr_fs {s t} [hs : sys.WF s] [ht : sys.WFTrans t] :
+sys.validTr (sym.fs s) t ↔ sys.validTr s (sym.ft' t) :=
+  ⟨validTr_ft'_of, validTr_fs_of⟩
+
+theorem validTr_fs' {s t} [hs : sys.WF s] [ht : sys.WFTrans t] :
+sys.validTr (sym.fs' s) t ↔ sys.validTr s (sym.ft t) :=
+  ⟨validTr_ft_of, validTr_fs'_of⟩
+
+theorem validTr_ft {s t} [hs : sys.WF s] [ht : sys.WFTrans t] :
+sys.validTr s (sym.ft t) ↔ sys.validTr (sym.fs' s) t :=
+  ⟨validTr_fs'_of, validTr_ft_of⟩
+
+theorem validTr_ft' {s t} [hs : sys.WF s] [ht : sys.WFTrans t] :
 sys.validTr s (sym.ft' t) ↔ sys.validTr (sym.fs s) t :=
   ⟨validTr_fs_of, validTr_ft'_of⟩
 
-@[simp] theorem hasTr_fs {s} [hs : sys.WF s] :
-sys.hasTr (sym.fs s) ↔ sys.hasTr s := Raw₀.hasTr_fs
+@[simp]
+theorem hasTr_fs {s} [hs : sys.WF s] : sys.hasTr (sym.fs s) ↔ sys.hasTr s := by
+  constructor <;> rintro ⟨t, h⟩ <;> have ht := wfTrans_of_validTr h
+  · use sym.ft' t; simpa [validTr_ft']
+  · use sym.ft t; simpa [validTr_ft]
 
 @[simp]
 theorem hasTr_fs' {s} [hs : sys.WF s] :
-sys.hasTr (sym.fs' s) ↔ sys.hasTr s := Raw₀.hasTr_fs'
+sys.hasTr (sym.fs' s) ↔ sys.hasTr s := by
+  constructor <;> rintro ⟨t, h⟩ <;> have ht := wfTrans_of_validTr h
+  · use sym.ft t; simpa [validTr_ft]
+  · use sym.ft' t; simpa [validTr_ft']
+
+#check 0 #exit
 
 @[simp]
-def simFn (sym : Raw sys) (f : S → T) (s : S) : T :=
-  sym.toRaw₀.simFn f s
+def simFn (sym : Symmetry sys) (f : S → T) (s : S) : T :=
+  sym.simFn f s
 
 instance {f} [hf : sys.SimFn f] : sys.SimFn (sym.simFn f) := by
   unfold simFn; infer_instance
